refactor(Untyped): `Star` relationships

TTFPI/Basic.lean
@@ -10,3 +10,24 @@ macro_rules | `($x ≡ $y) => `(binrel% Eq $x $y)
 
 unsafe instance {α : Type u} [ToString α] : ToString (Multiset α) where
   toString s := toString (s.unquot.map toString)
+
+inductive Star {α : Type u} (R : α → α → Prop) : α → α → Prop where
+| zero (a : α) : Star R a a
+| step {a b c : α} : R a b → Star R b c → Star R a c
+
+namespace Star
+
+variable {α b c : Type u}
+variable {R : α → α → Prop}
+
+@[refl]
+theorem refl (a : α) : Star R a a := zero a
+
+@[trans]
+theorem trans {a b c : α} : Star R a b → Star R b c → Star R a c := by
+  intro hlm hmn
+  induction hlm with
+  | zero => exact hmn
+  | step hlm' _ IH => exact step hlm' (IH hmn)
+
+end Star
